laxing generic code

crypto/bignum/Hacl.Bignum.fst
@@ -1,5 +1,6 @@
 module Hacl.Bignum
 
+open FStar.Mul
 open FStar.HyperStack
 open FStar.Buffer
 
@@ -15,56 +16,98 @@ open Hacl.Bignum.Crecip
 
 module U32 = FStar.UInt32
 
-#set-options "--lax"
 
 val fsum:
   a:felem ->
-  b:felem ->
+  b:felem{disjoint a b} ->
   Stack unit
-    (requires (fun _ -> True))
-    (ensures (fun _ _ _ -> true))
+    (requires (fun h -> live h a /\ live h b
+      /\ red_c h a len /\ red_c h b len))
+    (ensures (fun h0 _ h1 -> live h0 a /\ live h0 b /\ red_c h0 a len /\ red_c h0 b len
+      /\ live h1 a /\ modifies_1 a h0 h1
+      /\ eval h1 a = eval h0 a + eval h0 b))
 let fsum a b =
-  fsum_ a b clen
+  let h0 = ST.get() in
+  fsum_ a b clen;
+  let h1 = ST.get() in
+  assume (eval h1 a = eval h0 a + eval h0 b)
 
+#set-options "--initial_fuel 0 --max_fuel 0"
 
 val fdifference:
   a:felem ->
-  b:felem ->
+  b:felem{disjoint a b} ->
   Stack unit
-    (requires (fun _ -> True))
-    (ensures (fun _ _ _ -> true))
+    (requires (fun h -> live h a /\ live h b /\ add_zero_pre (as_seq h b)
+      /\ Hacl.Bignum.Fdifference.Spec.gte_limbs (as_seq h a) (add_zero_spec (as_seq h b)) len))
+    (ensures (fun h0 _ h1 -> live h0 a /\ live h0 b
+      /\ live h1 a /\ modifies_1 a h0 h1
+      /\ eval h1 a % prime = (eval h0 b - eval h0 a) % prime ))
 let fdifference a b =
-  add_zero b;
-  fdifference_ a b clen
+  let hinit = ST.get() in
+  push_frame();
+  let h0 = ST.get() in
+  let tmp = create limb_zero clen in
+  blit b 0ul tmp 0ul clen;
+  let h = ST.get() in
+  Hacl.Bignum.Fproduct.Spec.lemma_whole_slice (as_seq h b);
+  Hacl.Bignum.Fproduct.Spec.lemma_whole_slice (as_seq h tmp);
+  FStar.Seq.lemma_eq_intro (as_seq h b) (as_seq h tmp);
+  add_zero tmp;
+  fdifference_ a tmp clen;
+  let h1 = ST.get() in
+  pop_frame();
+  let hfin = ST.get() in
+  assume (eval hfin a % prime = (eval hinit b - eval hinit a) % prime)
 
+open Hacl.Bignum.Fscalar.Spec
+open Hacl.Bignum.Fproduct.Spec
 
 val fscalar:
   a:felem ->
-  b:felem ->
+  b:felem{disjoint a b} ->
   s:limb ->
   Stack unit
-    (requires (fun _ -> True))
-    (ensures (fun _ _ _ -> true))
+    (requires (fun h -> live h b /\ live h a
+      /\ carry_wide_pre (fscalar_spec (Seq.create len wide_zero) (as_seq h b) s len) 0
+      /\ reduce_wide_pre (carry_wide_spec (fscalar_spec (Seq.create len wide_zero) (as_seq h b) s len) 0)
+      /\ copy_from_wide_pre (reduce_wide_spec (carry_wide_spec (fscalar_spec (Seq.create len wide_zero) (as_seq h b) s len) 0)) ))
+    (ensures (fun h0 _ h1 -> live h0 a /\ live h0 b /\ modifies_1 a h0 h1 /\ live h1 a
+      /\ eval h1 a = eval h0 b * v s))
 let fscalar output b s =
+  let hinit = ST.get() in
   push_frame();
+  let h0 = ST.get() in
   let tmp = create wide_zero clen in
   fscalar tmp b s;
   carry_wide_ tmp 0ul;
   reduce_wide tmp;
   copy_from_wide_ output tmp clen;
-  pop_frame()
+  let h1 = ST.get() in
+  pop_frame();
+  let hfin = ST.get() in
+  assume (eval hfin output = eval hinit b * v s)
 
 
 val fmul:
   output:felem ->
-  a:felem ->
-  b:felem ->
+  a:felem{disjoint output a} ->
+  b:felem{disjoint output b} ->
   Stack unit
-    (requires (fun _ -> True))
-    (ensures (fun _ _ _ -> true))
+    (requires (fun h -> live h output /\ live h a /\ live h b
+      /\ fmul_pre (as_seq h a) (as_seq h b)))
+    (ensures (fun h0 _ h1 -> live h0 output /\ live h0 output /\ live h0 a /\ live h0 b 
+      /\ modifies_1 output h0 h1 /\ live h1 output
+      /\ eval h1 output % prime = (eval h0 a * eval h0 b) % prime
+      ))
 let fmul output a b =
-  fmul output a b
+  let h0 = ST.get() in
+  fmul output a b;
+  let h1 = ST.get() in
+  assume (eval h1 output % prime = (eval h0 a * eval h0 b) % prime)
 
+
+#set-options "--lax"
 
 val fsquare_times:
   output:felem ->
