crypto/bignum/Hacl.EC.Ladder.fst
@@ -6,7 +6,7 @@ open FStar.HyperStack
 open FStar.Ghost
 open FStar.Buffer
 
-
+open Hacl.Bignum.Constants
 open Hacl.Bignum.Parameters
 open Hacl.Bignum.Limb
 open Hacl.EC.Point
@@ -37,7 +37,7 @@ val cmult_small_loop:
     (requires (fun h -> true))
     (ensures (fun h0 _ h1 -> true))
 (* let rec cmult_small_loop nqx nqz nqpqx nqpqz nqx2 nqz2 nqpqx2 nqpqz2 q byte i = *)
-let rec cmult_small_loop nq nqpq nq2 nqpq2 q byte i =
+let rec cmult_small_loop nq nqpq nq2 nqpq2 q byt i =
   let nqx = getx nq in
   let nqz = getz nq in
   let nqpqx = getx nqpq in
@@ -46,9 +46,9 @@ let rec cmult_small_loop nq nqpq nq2 nqpq2 q byte i =
   let nqz2 = getz nq2 in
   let nqpqx2 = getx nqpq2 in
   let nqpqz2 = getz nqpq2 in
-  if (U32 (i =^ 0ul)) then ()
+  if (U32.(i =^ 0ul)) then ()
   else (
-    let bit = byte_to_limb (H8 (byte >>^ 7ul)) in
+    let bit = byte_to_limb (H8.(byt >>^ 7ul)) in
     (* swap_conditional nqx nqpqx bit; *)
     (* swap_conditional nqz nqpqz bit; *)
     swap_conditional nq nqpq bit;
@@ -69,9 +69,9 @@ let rec cmult_small_loop nq nqpq nq2 nqpq2 q byte i =
     let t = nqpqz in
     let nqpqz = nqpqz2 in
     let nqpqz2 = t in
-    let byte = H8 (byte <<^ 1ul) in
-    (* cmult_small_loop nqx nqz nqpqx nqpqz nqx2 nqz2 nqpqx2 nqpqz2 q byte (U32 (i -^ 1ul)) *)
-    cmult_small_loop nq nqpq nq2 nqpq2 q byte (U32 (i -^ 1ul))
+    let byt = H8.(byt <<^ 1ul) in
+    (* cmult_small_loop nqx nqz nqpqx nqpqz nqx2 nqz2 nqpqx2 nqpqz2 q byt (U32 (i -^ 1ul)) *)
+    cmult_small_loop nq nqpq nq2 nqpq2 q byt (U32.(i -^ 1ul))
   )
 
 
@@ -81,38 +81,34 @@ val cmult_big_loop:
   (* nqpqx:felem -> nqpqz:felem -> *)
   (* nqx2:felem -> nqz2:felem -> *)
   (* nqpqx2:felem -> nqpqz2:felem -> *)
-  nq:felem ->
-  nqpq:felem ->
-  nq2:felem ->
-  nqpq2:felem ->
-  q:felem -> i:U32.t ->
+  nq:point ->
+  nqpq:point ->
+  nq2:point ->
+  nqpq2:point ->
+  q:point ->
+  i:U32.t ->
   Stack unit
     (requires (fun h -> true))
     (ensures (fun h0 _ h1 -> true))
 (* let rec cmult_big_loop n nqx nqz nqpqx nqpqz nqx2 nqz2 nqpqx2 nqpqz2 q i = *)
 let rec cmult_big_loop n nq nqpq nq2 nqpq2 q i =
-  if (U32 (i =^ 0ul)) then ()
+  if (U32.(i =^ 0ul)) then ()
   else (
-    let i = U32 (i -^ 1ul) in
+    let i = U32.(i -^ 1ul) in
     let byte = n.(i) in
     cmult_small_loop nq nqpq nq2 nqpq2 q byte 8ul;
     cmult_big_loop n nq nqpq nq2 nqpq2 q i
   )
 
 
-val cmult:
-  (* resultx:felem -> resultz:felem -> *)
-  result:felem ->
-  n:uint8_p{length n = 32} ->
-  q:felem ->
-  Stack unit
-    (requires (fun _ -> true))
-    (ensures (fun _ _ _ -> true))
-    (* (requires (fun h -> live h resultx /\ live h resultz /\ live h n /\ live h q)) *)
-    (* (ensures (fun h0 _ h1 -> modifies_2 resultx resultz h0 h1 /\ live h1 resultx /\ live h1 resultz)) *)
+val cmult: result:point -> (* point at infinity when starting *)
+  scalar:uint8_p{length scalar = keylen} ->
+  q:point -> Stack unit
+  (requires (fun _ -> true))
+  (ensures (fun _ _ _ -> true))
 let cmult result n q =
   push_frame();
-  let buf = create zero 40ul in
+  (* let buf = create zero 40ul in *)
   (* let nqpqx  = Buffer.sub buf 0ul  5ul in *)
   (* let nqpqz  = Buffer.sub buf 5ul  5ul in *)
   (* let nqx    = Buffer.sub buf 10ul 5ul in *)
@@ -121,26 +117,72 @@ let cmult result n q =
   (* let nqpqz2 = Buffer.sub buf 25ul 5ul in *)
   (* let nqx2   = Buffer.sub buf 30ul 5ul in *)
   (* let nqz2   = Buffer.sub buf 35ul 5ul in *)
-  let nqpq  = Buffer.sub buf 0ul  10ul in
-  let nq    = Buffer.sub buf 10ul 10ul in
-  let nqpq2 = Buffer.sub buf 20ul 10ul in
-  let nq2   = Buffer.sub buf 30ul 10ul in
-  let nqpqx = getx nqpq in
-  let nqpqz = getz nqpq in
-  let nqx = getx nq in
-  let nqz = getz nq in
-  let nqpqx2 = getx nqpq2 in
-  let nqpqz2 = getz nqpq2 in
-  let nqx2 = getx nq2 in
-  let nqz2 = getz nq2 in
-  nqpqz.(0ul) <- one;
-  nqx.(0ul) <- one;
-  nqpqz2.(0ul) <- one;
-  nqz2.(0ul) <- one;
-  blit q 0ul nqpqx 0ul 5ul;
+  let nq    = result in
+  let nqpq  = Hacl.EC.Format.alloc_point () in
+  let nqpq2 = Hacl.EC.Format.alloc_point () in
+  let nq2   = Hacl.EC.Format.alloc_point () in
+  (* let nqpqx = getx nqpq in *)
+  (* let nqpqz = getz nqpq in *)
+  (* let nqx = getx nq in *)
+  (* let nqz = getz nq in *)
+  (* let nqpqx2 = getx nqpq2 in *)
+  (* let nqpqz2 = getz nqpq2 in *)
+  (* let nqx2 = getx nq2 in *)
+  (* let nqz2 = getz nq2 in *)
+  (* nqpqz.(0ul) <- one; *)
+  (* nqx.(0ul) <- one; *)
+  (* nqpqz2.(0ul) <- one; *)
+  (* nqz2.(0ul) <- one; *)
+  (* blit q 0ul nqpqx 0ul 5ul; *)
+  Hacl.EC.Point.copy nqpq q;
   (* cmult_big_loop n nqx nqz nqpqx nqpqz nqx2 nqz2 nqpqx2 nqpqz2 q 32ul; *)
   cmult_big_loop n nq nqpq nq2 nqpq2 q 32ul;
   copy result nq;
   (* blit nqx 0ul resultx 0ul 5ul; *)
   (* blit nqz 0ul resultz 0ul 5ul; *)
   pop_frame()
+
+(* val cmult: *)
+(*   (\* resultx:felem -> resultz:felem -> *\) *)
+(*   result:felem -> *)
+(*   n:uint8_p{length n = 32} -> *)
+(*   q:felem -> *)
+(*   Stack unit *)
+(*     (requires (fun _ -> true)) *)
+(*     (ensures (fun _ _ _ -> true)) *)
+(*     (\* (requires (fun h -> live h resultx /\ live h resultz /\ live h n /\ live h q)) *\) *)
+(*     (\* (ensures (fun h0 _ h1 -> modifies_2 resultx resultz h0 h1 /\ live h1 resultx /\ live h1 resultz)) *\) *)
+(* let cmult result n q = *)
+(*   push_frame(); *)
+(*   let buf = create zero 40ul in *)
+(*   (\* let nqpqx  = Buffer.sub buf 0ul  5ul in *\) *)
+(*   (\* let nqpqz  = Buffer.sub buf 5ul  5ul in *\) *)
+(*   (\* let nqx    = Buffer.sub buf 10ul 5ul in *\) *)
+(*   (\* let nqz    = Buffer.sub buf 15ul 5ul in *\) *)
+(*   (\* let nqpqx2 = Buffer.sub buf 20ul 5ul in *\) *)
+(*   (\* let nqpqz2 = Buffer.sub buf 25ul 5ul in *\) *)
+(*   (\* let nqx2   = Buffer.sub buf 30ul 5ul in *\) *)
+(*   (\* let nqz2   = Buffer.sub buf 35ul 5ul in *\) *)
+(*   let nqpq  = Buffer.sub buf 0ul  10ul in *)
+(*   let nq    = Buffer.sub buf 10ul 10ul in *)
+(*   let nqpq2 = Buffer.sub buf 20ul 10ul in *)
+(*   let nq2   = Buffer.sub buf 30ul 10ul in *)
+(*   let nqpqx = getx nqpq in *)
+(*   let nqpqz = getz nqpq in *)
+(*   let nqx = getx nq in *)
+(*   let nqz = getz nq in *)
+(*   let nqpqx2 = getx nqpq2 in *)
+(*   let nqpqz2 = getz nqpq2 in *)
+(*   let nqx2 = getx nq2 in *)
+(*   let nqz2 = getz nq2 in *)
+(*   nqpqz.(0ul) <- one; *)
+(*   nqx.(0ul) <- one; *)
+(*   nqpqz2.(0ul) <- one; *)
+(*   nqz2.(0ul) <- one; *)
+(*   blit q 0ul nqpqx 0ul 5ul; *)
+(*   (\* cmult_big_loop n nqx nqz nqpqx nqpqz nqx2 nqz2 nqpqx2 nqpqz2 q 32ul; *\) *)
+(*   cmult_big_loop n nq nqpq nq2 nqpq2 q 32ul; *)
+(*   copy result nq; *)
+(*   (\* blit nqx 0ul resultx 0ul 5ul; *\) *)
+(*   (\* blit nqz 0ul resultz 0ul 5ul; *\) *)
+(*   pop_frame() *)
