crypto/bignum/x25519/Hacl.Bignum.Constants.fst
@@ -4,3 +4,7 @@ inline_for_extraction let prime = assert_norm(pow2 255 > 19); pow2 255 - 19
 inline_for_extraction let word_size = 64
 inline_for_extraction let len = 5
 inline_for_extraction let limb_size = 51
+inline_for_extraction let keylen = 32
+inline_for_extraction let limb = Hacl.UInt64.t
+inline_for_extraction let wide = Hacl.UInt128.t
+inline_for_extraction let a24 = assert_norm(121665 < pow2 64); 121665uL
