crypto/bignum/x25519/Hacl.EC.Point.fst
@@ -12,16 +12,57 @@ open Hacl.Bignum
 
 module U32 = FStar.UInt32
 
-let plen = 10
-let cplen = 10ul
+(* let plen = 10 *)
+(* let cplen = 10ul *)
+
+let point =
+  let _ = () in
+  b:buffer limb{length b = 10}
 
 let getx p = Buffer.sub p 0ul 5ul
 let gety p = Buffer.sub p 0ul 5ul
 let getz p = Buffer.sub p 5ul 5ul
 
-let live_coords h x y z = live h x /\ live h z
+let live_coords h x y z =
+  let _ = () in
+  live h x /\ live h z
 
-let live h p = live_coords h (getx p) (gety p) (getz p)
+let live h p =
+  let _ = () in
+  live_coords h (getx p) (gety p) (getz p)
 
-let make x y z = admit()
+let make_pre x y z =
+  let _ = () in
+  content x == content z /\ max_length x == max_length z /\ idx z = idx x + length x
 
+let make x y z = join x z
+
+let valid h p = admit()
+
+
+private val swap_conditional_: a:felem -> b:felem -> swap:limb -> ctr:U32.t ->
+  Stack unit
+    (requires (fun h -> live h a /\ live h b))
+    (ensures (fun h0 _ h1 -> modifies_2 a b h0 h1 /\ live h1 a /\ live h1 b))
+private let rec swap_conditional_ a b swap ctr =
+  if U32.(ctr =^ 0ul) then ()
+  else (
+    let i = U32.(ctr -^ 1ul) in
+    let ai = a.(i) in
+    let bi = b.(i) in
+    let x = swap &^ (ai ^^ bi) in
+    let ai = ai ^^ x in
+    let bi = bi ^^ x in
+    a.(i) <- ai;
+    b.(i) <- bi;
+    swap_conditional_ a b swap i
+  )
+
+let swap_conditional a b iswap =
+  let swap = limb_zero -^ iswap in
+  swap_conditional_ (getx a) (getx b) swap clen;
+  swap_conditional_ (getz a) (getz b) swap clen
+
+let copy output input =
+  blit (getx input) 0ul (getx output) 0ul clen;
+  blit (getz input) 0ul (getz output) 0ul clen
