crypto/bignum/Hacl.EC.fst
@@ -1,0 +1,36 @@
+module Hacl.EC
+
+open FStar.Mul
+open FStar.HyperStack
+open FStar.Ghost
+open FStar.Buffer
+
+open Hacl.Bignum.Constants
+open Hacl.Bignum.Parameters
+open Hacl.Bignum.Limb
+open Hacl.EC.Point
+open Hacl.EC.Format
+open Hacl.EC.Ladder
+
+module U32 = FStar.UInt32
+module H8 = Hacl.UInt8
+
+
+val crypto_scalarmult:
+  mypublic:uint8_p{length mypublic = 32} ->
+  secret:uint8_p{length secret = 32} ->
+  basepoint:uint8_p{length basepoint = 32} ->
+  Stack unit
+    (requires (fun h -> Buffer.live h mypublic /\ Buffer.live h secret /\ Buffer.live h basepoint))
+    (ensures (fun h0 _ h1 -> Buffer.live h1 mypublic /\ modifies_1 mypublic h0 h1))
+let crypto_scalarmult mypublic secret basepoint =
+  push_frame();  
+  let q  = point_of_scalar basepoint in
+  let nq = Hacl.EC.Format.point_inf () in // Storage point
+  let x = getx nq in
+  let z = getz nq in
+  let zmone = Buffer.create limb_zero clen in
+  let scalar = format_secret secret in
+  cmult nq scalar q;
+  scalar_of_point mypublic nq;
+  pop_frame()
