crypto/bignum/x25519/Blah.fst
@@ -1,5 +1,0 @@
-module Blah
-
-open Test
-
-let test () = assert(x = 3)
