crypto/bignum/x25519/Hacl.EC.AddAndDouble.fst
@@ -3,8 +3,13 @@ module Hacl.EC.AddAndDouble
 open FStar.HyperStack
 open FStar.Buffer
 
+open Hacl.Bignum.Constants
+open Hacl.Bignum.Parameters
+open Hacl.Bignum
+open Hacl.EC.Point
 
-let fmonty x2 z2 x3 z3 x z xprime zprime qmqp =
+let fmonty pp ppq p pq qmqp =
+  let qx = getx qmqp in
   let x2 = getx pp in
   let z2 = getz pp in
   let x3 = getx ppq in
@@ -14,7 +19,7 @@ let fmonty x2 z2 x3 z3 x z xprime zprime qmqp =
   let xprime  = getx pq in
   let zprime  = getz pq in
   push_frame();
-  let buf = create zero_64 40ul in
+  let buf = create limb_zero 40ul in
   let origx      = Buffer.sub buf 0ul  5ul in
   let origxprime = Buffer.sub buf 5ul  5ul in
   let zzz        = Buffer.sub buf 10ul 5ul in
@@ -36,12 +41,12 @@ let fmonty x2 z2 x3 z3 x z xprime zprime qmqp =
   fdifference zzprime origxprime; // zzprime <- sub
   fsquare_times x3 xxprime 1ul; // sum sum
   fsquare_times zzzprime zzprime 1ul; // sub sub 
-  fmul z3 zzzprime qmqp;
+  fmul z3 zzzprime qx;
   fsquare_times xx x 1ul; // sum red
   fsquare_times zz z 1ul; // red sub 
   fmul x2 xx zz; // red red
   fdifference zz xx; // red red
-  fscalar_product zzz zz (uint64_to_sint64 121665uL);
+  fscalar zzz zz (uint64_to_limb Hacl.Bignum.Constants.a24);
   fsum zzz xx; // red red
   fmul z2 zz zzz;
   pop_frame()
