crypto/bignum/x25519/Hacl.EC.Format.fst
@@ -1,0 +1,198 @@
+module Hacl.EC.Format
+
+
+open FStar.Mul
+open FStar.HyperStack
+open FStar.Ghost
+open FStar.Buffer
+
+open Hacl.Cast
+open Hacl.Bignum.Constants
+open Hacl.Bignum.Parameters
+open Hacl.Bignum.Limb
+open Hacl.EC.Point
+
+private inline_for_extraction let zero_8 = uint8_to_sint8 0uy
+
+let point_inf () =
+  let buf = create limb_zero 10ul in
+  let x = Buffer.sub buf 0ul 5ul in
+  let y = Buffer.sub buf 0ul 5ul in
+  let z = Buffer.sub buf 5ul 5ul in
+  x.(0ul) <- limb_one;
+  let p = make x y z in
+  p
+
+
+let alloc_point () =
+  let buf = create limb_zero 10ul in
+  let x = Buffer.sub buf 0ul 5ul in
+  let y = Buffer.sub buf 0ul 5ul in
+  let z = Buffer.sub buf 5ul 5ul in
+  make x y z
+
+
+private val load64_le:
+  b:uint8_p{length b >= 8} ->
+  Stack limb
+    (requires (fun h -> Buffer.live h b))
+    (ensures  (fun h0 _ h1 -> h0 == h1))
+private let load64_le b =
+  let b0 = b.(0ul) in
+  let b1 = b.(1ul) in
+  let b2 = b.(2ul) in
+  let b3 = b.(3ul) in
+  let b4 = b.(4ul) in
+  let b5 = b.(5ul) in
+  let b6 = b.(6ul) in
+  let b7 = b.(7ul) in
+  Hacl.Bignum.Limb.(
+    sint8_to_sint64 b0
+    |^ (sint8_to_sint64 b1 <<^ 8ul)
+    |^ (sint8_to_sint64 b2 <<^ 16ul)
+    |^ (sint8_to_sint64 b3 <<^ 24ul)
+    |^ (sint8_to_sint64 b4 <<^ 32ul)
+    |^ (sint8_to_sint64 b5 <<^ 40ul)
+    |^ (sint8_to_sint64 b6 <<^ 48ul)
+    |^ (sint8_to_sint64 b7 <<^ 56ul)
+  )
+
+
+private val store64_le:
+  b:uint8_p{length b >= 8} ->
+  z:limb ->
+  Stack unit
+    (requires (fun h -> Buffer.live h b))
+    (ensures  (fun h0 _ h1 -> modifies_1 b h0 h1 /\ Buffer.live h1 b))
+private let store64_le b z =
+  let open Hacl.Bignum.Limb in
+  b.(0ul) <- sint64_to_sint8 z;
+  b.(1ul) <- sint64_to_sint8 (z >>^ 8ul);
+  b.(2ul) <- sint64_to_sint8 (z >>^ 16ul);
+  b.(3ul) <- sint64_to_sint8 (z >>^ 24ul);
+  b.(4ul) <- sint64_to_sint8 (z >>^ 32ul);
+  b.(5ul) <- sint64_to_sint8 (z >>^ 40ul);
+  b.(6ul) <- sint64_to_sint8 (z >>^ 48ul);
+  b.(7ul) <- sint64_to_sint8 (z >>^ 56ul)
+  
+
+private val fexpand: output:felem -> input:uint8_p{length input = 32} -> Stack unit
+  (requires (fun h -> Buffer.live h output /\ Buffer.live h input))
+  (ensures (fun h0 _ h1 -> Buffer.live h1 output /\ modifies_1 output h0 h1))
+private let fexpand output input =
+  let mask_51 = uint64_to_limb 0x7ffffffffffffuL in
+  let i0 = load64_le (Buffer.sub input 0ul 8ul) in
+  let i1 = load64_le (Buffer.sub input 6ul 8ul) in
+  let i2 = load64_le (Buffer.sub input 12ul 8ul) in
+  let i3 = load64_le (Buffer.sub input 19ul 8ul) in
+  let i4 = load64_le (Buffer.sub input 24ul 8ul) in
+  let output0 = (i0         ) &^ mask_51 in
+  let output1 = (i1 >>^ 3ul ) &^ mask_51 in
+  let output2 = (i2 >>^ 6ul ) &^ mask_51 in
+  let output3 = (i3 >>^ 1ul ) &^ mask_51 in
+  let output4 = (i4 >>^ 12ul) &^ mask_51 in
+  output.(0ul) <- output0;
+  output.(1ul) <- output1;
+  output.(2ul) <- output2;
+  output.(3ul) <- output3;
+  output.(4ul) <- output4
+
+
+private val fcontract: output:uint8_p{length output = 32} -> input:felem -> Stack unit
+  (requires (fun h -> Buffer.live h output /\ Buffer.live h input))
+  (ensures (fun h0 _ h1 -> Buffer.live h1 output /\ modifies_1 output h0 h1))
+private let fcontract output input =
+  let mask_51 = uint64_to_limb 0x7ffffffffffffuL in
+  let nineteen = uint64_to_limb 19uL in
+  let t0 = input.(0ul) in
+  let t1 = input.(1ul) in
+  let t2 = input.(2ul) in
+  let t3 = input.(3ul) in
+  let t4 = input.(4ul) in
+  let t1 = t1 +%^ (t0 >>^ 51ul) in
+  let t0 = t0 &^ mask_51 in
+  let t2 = t2 +%^ (t1 >>^ 51ul) in
+  let t1 = t1 &^ mask_51 in
+  let t3 = t3 +%^ (t2 >>^ 51ul) in
+  let t2 = t2 &^ mask_51 in
+  let t4 = t4 +%^ (t3 >>^ 51ul) in
+  let t3 = t3 &^ mask_51 in
+  let t0 = t0 +^ (nineteen *%^ (t4 >>^ 51ul)) in
+  let t4 = t4 &^ mask_51 in
+  let t1 = t1 +%^ (t0 >>^ 51ul) in
+  let t0 = t0 &^ mask_51 in
+  let t2 = t2 +%^ (t1 >>^ 51ul) in
+  let t1 = t1 &^ mask_51 in
+  let t3 = t3 +%^ (t2 >>^ 51ul) in
+  let t2 = t2 &^ mask_51 in
+  let t4 = t4 +%^ (t3 >>^ 51ul) in
+  let t3 = t3 &^ mask_51 in
+  let t0 = t0 +^ (nineteen *%^ (t4 >>^ 51ul)) in
+  let t4 = t4 &^ mask_51 in
+  let t0 = t0 +%^ nineteen in
+  let t1 = t1 +%^ (t0 >>^ 51ul) in
+  let t0 = t0 &^ mask_51 in
+  let t2 = t2 +%^ (t1 >>^ 51ul) in
+  let t1 = t1 &^ mask_51 in
+  let t3 = t3 +%^ (t2 >>^ 51ul) in
+  let t2 = t2 &^ mask_51 in
+  let t4 = t4 +%^ (t3 >>^ 51ul) in
+  let t3 = t3 &^ mask_51 in
+  let t0 = t0 +^ (nineteen *%^ (t4 >>^ 51ul)) in
+  let t4 = t4 &^ mask_51 in
+  let two52 = uint64_to_sint64 0x8000000000000uL in
+  let t0 = t0 +%^ two52 -%^ nineteen in
+  let t1 = t1 +%^ two52 -%^ limb_one in
+  let t2 = t2 +%^ two52 -%^ limb_one in
+  let t3 = t3 +%^ two52 -%^ limb_one in
+  let t4 = t4 +%^ two52 -%^ limb_one in
+  let t1 = t1 +%^ (t0 >>^ 51ul) in
+  let t0 = t0 &^ mask_51 in
+  let t2 = t2 +%^ (t1 >>^ 51ul) in
+  let t1 = t1 &^ mask_51 in
+  let t3 = t3 +%^ (t2 >>^ 51ul) in
+  let t2 = t2 &^ mask_51 in
+  let t4 = t4 +%^ (t3 >>^ 51ul) in
+  let t3 = t3 &^ mask_51 in
+  let t4 = t4 &^ mask_51 in
+  let o0 = t0 |^ (t1 <<^ 51ul) in
+  let o1 = (t1 >>^ 13ul) |^ (t2 <<^ 38ul) in
+  let o2 = (t2 >>^ 26ul) |^ (t3 <<^ 25ul) in
+  let o3 = (t3 >>^ 39ul) |^ (t4 <<^ 12ul) in
+  store64_le (Buffer.sub output 0ul  8ul) o0;
+  store64_le (Buffer.sub output 8ul  8ul) o1;
+  store64_le (Buffer.sub output 16ul 8ul) o2;
+  store64_le (Buffer.sub output 24ul 8ul) o3
+
+
+let point_of_scalar scalar =
+  let buf = create limb_zero 10ul in
+  let x = Buffer.sub buf 0ul 5ul in
+  let y = Buffer.sub buf 0ul 5ul in
+  let z = Buffer.sub buf 5ul 5ul in
+  let p = make x y z in
+  fexpand x scalar;
+  z.(0ul) <- limb_one;
+  p
+
+let scalar_of_point scalar point =
+  push_frame();
+  let x = Hacl.EC.Point.getx point in
+  let z = Hacl.EC.Point.getz point in
+  let zmone = Buffer.create limb_zero clen in
+  Hacl.Bignum.crecip zmone z;
+  Hacl.Bignum.fmul z x zmone;
+  fcontract scalar z;
+  pop_frame()
+
+
+let format_secret secret =
+  let e   = create zero_8 32ul in
+  blit secret 0ul e 0ul 32ul;
+  let e0  = e.(0ul) in
+  let e31 = e.(31ul) in
+  let open Hacl.UInt8 in
+  let e0  = e0 &^ (uint8_to_sint8 248uy) in
+  let e31 = e31 &^ (uint8_to_sint8 127uy) in
+  let e31 = e31 |^ (uint8_to_sint8 64uy) in
+  e
