crypto/bignum/x25519/Test.fst
@@ -1,3 +1,0 @@
-module Test
-
-let x = 3
